models/queue2.bpl
@@ -1,0 +1,85 @@
+type Event = int;
+
+const unique $NULL: int;
+axiom $NULL == 0;
+
+const unique _ping: Event;
+const unique _pong: Event;
+
+var $Inbox: [int]Queue;
+
+type {:datatype} Queue;
+
+function {:constructor} $queue() : Queue;
+function {:constructor} $q_cons(e:Event, q:Queue) : Queue;
+
+function $q_first(Queue) returns (Event);
+function $q_tail(Queue) returns (Queue);
+function $q_length(Queue) returns (int);
+function $q_index(int, Queue) returns (Event);
+function $q_remove(int, Queue) returns (Queue);
+function $q_enqueue(Event, Queue) returns (Queue);
+
+axiom $q_length($queue()) == 0;
+axiom (forall e:Event, q:Queue :: $q_length($q_cons(e, q)) == 1 + $q_length(q));
+
+axiom (forall e:Event, q:Queue :: $q_first($queue()) == $NULL);
+axiom (forall e:Event, q:Queue :: $q_first($q_cons(e, q)) == e);
+
+axiom (forall e:Event, q:Queue :: $q_tail($queue()) == $queue());
+axiom (forall e:Event, q:Queue :: $q_tail($q_cons(e, q)) == q);
+
+axiom (forall i:int, q:Queue :: {$q_index(i, q)} $q_index(i, q) ==
+  if i == 0 then $q_first(q)
+  else $q_index(i - 1, $q_tail(q)));
+
+axiom (forall i:int, q:Queue :: {$q_remove(i, q)} $q_remove(i, q) ==
+  if i == 0 then $q_tail(q)
+  else $q_cons($q_first(q), $q_remove(i - 1, $q_tail(q))));
+
+axiom (forall e:Event, q:Queue :: {$q_enqueue(e, q)} $q_enqueue(e, q) ==
+  if q == $queue() then $q_cons(e, q)
+  else $q_cons($q_first(q), $q_enqueue(e, $q_tail(q))));
+
+
+// Test harness
+procedure {:entrypoint} Main();
+  modifies $Inbox;
+
+implementation {:entrypoint} Main()
+{
+  $main:
+    $Inbox[0] := $queue();
+    assert $q_length($Inbox[0]) == 0;
+    assert $q_first($Inbox[0]) == $NULL;
+
+    $Inbox[0] := $q_cons(_ping, $Inbox[0]);
+    assert $q_length($Inbox[0]) == 1;
+    assert $q_length($q_tail($Inbox[0])) == 0;
+    assert $q_first($Inbox[0]) == _ping;
+
+    $Inbox[0] := $q_cons(_pong, $Inbox[0]);
+    assert $q_length($Inbox[0]) == 2;
+    assert $q_first($Inbox[0]) == _pong;
+
+    assert $q_index(0, $Inbox[0]) == _pong;
+    assert $q_index(1, $Inbox[0]) == _ping;
+
+    $Inbox[0] := $q_remove(0, $Inbox[0]);
+    assert $q_index(0, $Inbox[0]) == _ping;
+
+    $Inbox[0] := $queue();
+    $Inbox[0] := $q_enqueue(_ping, $Inbox[0]);
+    assert $q_length($Inbox[0]) == 1;
+    assert $q_first($Inbox[0]) == _ping;
+
+    $Inbox[0] := $q_enqueue(_pong, $Inbox[0]);
+    $Inbox[0] := $q_enqueue(_pong, $Inbox[0]);
+    assert $q_length($Inbox[0]) == 3;
+    assert $q_first($Inbox[0]) == _ping;
+
+    $Inbox[0] := $q_remove(0, $Inbox[0]);
+    assert $q_index(0, $Inbox[0]) == _pong;
+
+    return;
+}
